code/Yazi.CRC32.fsti
@@ -1,0 +1,94 @@
+module Yazi.CRC32
+
+module B = LowStar.Buffer
+module Cast = FStar.Int.Cast
+module CB = LowStar.ConstBuffer
+module Ghost = FStar.Ghost
+module HS = FStar.HyperStack
+module U32 = FStar.UInt32
+module U64 = FStar.UInt64
+module U8 = FStar.UInt8
+module Seq = FStar.Seq
+module Spec = Spec.CRC32
+module ST = FStar.HyperStack.ST
+
+private type matrix_buf = B.lbuffer U32.t 32
+
+[@ (CPrologue "#ifndef YAZI_CRC32_TABLE_GEN")
+   (CEpilogue "#endif")]
+val crc32:
+    data: Ghost.erased (Seq.seq U8.t)
+  -> crc: U32.t
+  -> buf: CB.const_buffer U8.t
+  -> len: U32.t
+  -> ST.Stack U32.t
+  (requires fun h ->
+    CB.live h buf /\ CB.length buf == U32.v len /\
+    Spec.crc32_matched (Seq.length data) data crc true)
+  (ensures fun h0 res h1 ->
+    B.(modifies loc_none h0 h1) /\
+    Spec.crc32_matched
+      (Seq.length data + U32.v len)
+      (Seq.append data (CB.as_seq h1 buf)) res true)
+
+[@ (CPrologue "#ifndef YAZI_CRC32_TABLE_GEN")
+   (CEpilogue "#endif")]
+val crc32_combine64:
+    s1: Ghost.erased (Seq.seq U8.t)
+  -> s2: Ghost.erased (Seq.seq U8.t)
+  -> crc1: U32.t
+  -> crc2: U32.t
+  -> length: U64.t
+  -> ST.Stack U32.t
+    (requires fun h ->
+      Spec.crc32_matched (Seq.length s1) s1 crc1 true /\
+      Spec.crc32_matched (Seq.length s2) s2 crc2 true /\
+      U64.v length == Seq.length s2)
+    (ensures fun h0 res h1 ->
+      B.(modifies loc_none h0 h1) /\
+      Spec.crc32_matched (Seq.length s1 + Seq.length s2) (Seq.append s1 s2) res true)
+
+[@ (CPrologue "#ifndef YAZI_CRC32_TABLE_GEN")
+   (CEpilogue "#endif")]
+let crc32_combine (s1 s2: Ghost.erased (Seq.seq U8.t)) (crc1 crc2 length: U32.t):
+ST.Stack U32.t
+(requires fun h ->
+  Spec.crc32_matched (Seq.length s1) s1 crc1 true /\
+  Spec.crc32_matched (Seq.length s2) s2 crc2 true /\
+  U32.v length == Seq.length s2)
+(ensures fun h0 res h1 ->
+  B.(modifies loc_none h0 h1) /\
+  Spec.crc32_matched (Seq.length s1 + Seq.length s2) (Seq.append s1 s2) res true) =
+  crc32_combine64 s1 s2 crc1 crc2 (Cast.uint32_to_uint64 length)
+
+[@ (CPrologue "#ifdef YAZI_CRC32_TABLE_GEN")
+   (CEpilogue "#endif")]
+val gen_crc32_table:
+    t8: B.lbuffer U32.t 256
+  -> t16: B.lbuffer U32.t 256
+  -> t24: B.lbuffer U32.t 256
+  -> t32: B.lbuffer U32.t 256
+  -> ST.Stack unit
+  (requires fun h ->
+    B.live h t8 /\ B.live h t16 /\ B.live h t24 /\ B.live h t32 /\
+    B.disjoint t8 t16 /\ B.disjoint t8 t24 /\ B.disjoint t8 t32 /\
+    B.disjoint t16 t24 /\ B.disjoint t16 t32 /\ B.disjoint t24 t32)
+  (ensures fun h0 _ h1 ->
+    B.modifies 
+      (B.loc_buffer t8 `B.loc_union`
+      B.loc_buffer t16 `B.loc_union`
+      B.loc_buffer t24 `B.loc_union`
+      B.loc_buffer t32)
+      h0 h1 /\
+    Spec.table_correct 8 h1 (CB.of_buffer t8) /\
+    Spec.table_correct 16 h1 (CB.of_buffer t16) /\
+    Spec.table_correct 24 h1 (CB.of_buffer t24) /\
+    Spec.table_correct 32 h1 (CB.of_buffer t32))
+
+[@ (CPrologue "#ifdef YAZI_CRC32_TABLE_GEN")
+   (CEpilogue "#endif")]
+val gen_matrix_table:
+    buf: Spec.matrix_buf
+  -> ST.Stack unit
+  (requires fun h -> B.live h buf)
+  (ensures fun h0 _ h1 -> B.modifies (B.loc_buffer buf) h0 h1 /\ Spec.is_matrix_buf h1 8 buf)
